LeanNanoLlvm/Refinement/Test.lean
@@ -1,0 +1,52 @@
+import LeanNanoLlvm.Refinement
+import LeanNanoLlvm.AST.Syntax
+
+namespace LeanNanoLlvm.Refinement
+
+open LeanNanoLlvm
+open Semantics
+open AST.Syntax
+
+open scoped LeanNanoLlvm.AST.Syntax in
+def addDef : @AST.Definition 512 := [llvm-definition|
+  define i8 @f(i8 %a, i8 %b) {
+  entry:
+    %x = add i8 %a, %b
+    ret i8 %x
+  }
+]
+
+theorem addDef_refines_itself : addDef ⊑ addDef := by
+  intro args st retval h
+  exact h
+
+open scoped LeanNanoLlvm.AST.Syntax in
+def retAddX0Def : @AST.Definition 512 := [llvm-definition|
+  define i8 @f(i8 %x) {
+  entry:
+    %x = add i8 %x, 0
+    ret i8 %x
+  }
+]
+
+open scoped LeanNanoLlvm.AST.Syntax in
+def retXDef : @AST.Definition 512 := [llvm-definition|
+  define i8 @f(i8 %x) {
+  entry:
+    ret i8 %x
+  }
+]
+
+private theorem intw_add_zero (x : Semantics.IntW 8) :
+    (do let y ← x; pure (y + (0 : BitVec 8))) = x := by
+  cases x with
+  | ofOption o =>
+    cases o <;> simp
+
+
+theorem ret_add_x_0_refines_ret_x : retAddX0Def ⊑ retXDef := by
+  intro args undefs retval h
+  sorry
+
+
+end LeanNanoLlvm.Refinement
