LeanNanoLlvm/Semantics.lean
@@ -1,3 +1,4 @@
 import LeanNanoLlvm.Semantics.Semantics
 import LeanNanoLlvm.Semantics.State
 import LeanNanoLlvm.Semantics.Denote
+import LeanNanoLlvm.Semantics.Wellformed
