LeanNanoLlvm/Semantics/Wellformed.lean
@@ -1,0 +1,68 @@
+import LeanNanoLlvm.Semantics.Denote
+
+namespace LeanNanoLlvm
+namespace AST
+
+variable {φ : Nat}
+
+inductive Declaration.WellFormed (decl : @Declaration φ) : Prop where
+  | mk :
+    decl.type.asFunction? = some ⟨retTy, argTys⟩ →
+    retTy.isVoid? ∨ (retTy.asRet? = some retRetTy ∧ retRetTy.asInt?.isSome) →
+    (∀ argTy ∈ argTys, argTy.asFunction?.isNone) →
+    WellFormed decl
+
+inductive Definition.WellFormed (defn : @Definition φ) : Prop where
+  | mk : defn.prototype.WellFormed → WellFormed defn
+
+theorem declaration_wellFormed_iff (decl : @Declaration φ) :
+    decl.WellFormed ↔
+      ∃ retTy argTys, decl.type = LlvmType.function retTy argTys
+      ∧ (retTy.isVoid? = true ∨ (∃ retRetTy, retTy.asRet? = some retRetTy ∧ retRetTy.asInt?.isSome))
+      ∧ (∀ argTy ∈ argTys, argTy.asFunction?.isNone)
+  := by
+  constructor
+  . intro h
+    cases h with
+    | mk h =>
+      aesop
+  . simp
+    rintro retTy argTys htype (hret1|(⟨retRetTy, ⟨hret2, hret3⟩⟩)) hargs
+    constructor
+    . simp_all
+      constructor
+      . cases retTy
+        . rfl
+        . contradiction
+      . rfl
+    . left
+      simp
+    . simp_all
+    . exact (LlvmType.i1)
+    . constructor
+      . simp_all
+        constructor
+        . rfl
+        . rfl
+      . right
+        simp_all
+        constructor
+        . rfl
+        . simp_all
+      . simp_all
+
+
+theorem definition_wellFormed_iff (defn : @Definition φ) :
+    defn.WellFormed ↔ defn.prototype.WellFormed := by
+  constructor
+  . intro h
+    cases h with
+    | mk hproto =>
+      exact hproto
+  . intro hproto
+    constructor
+    . exact hproto
+
+end AST
+
+end LeanNanoLlvm
